theories/Sep/Spec.v
@@ -152,28 +152,8 @@ Module Assertions
 
   Instance instantiate_formula_laws : InstLaws Formula Prop.
   Proof.
-    constructor; auto.
-    intros Σ Σ' ζ ι t.
-    induction t.
-    - cbn. f_equal. apply inst_subst.
-    - unfold subst, sub_formula, inst at 1 2, instantiate_formula, inst_formula.
-      f_equal.
-      apply inst_subst.
-    - unfold subst, sub_formula, inst at 1 2, instantiate_formula, inst_formula.
-      f_equal.
-      eapply inst_subst.
-    - unfold subst, sub_formula, inst at 1 2, instantiate_formula, inst_formula.
-      f_equal; eapply inst_subst.
-    - unfold subst, sub_formula, inst at 1 2, instantiate_formula, inst_formula.
-      f_equal; eapply inst_subst.
-    - unfold subst, sub_formula, inst at 1 2, instantiate_formula, inst_formula.
-      f_equal; eapply inst_subst.
-    - unfold subst, sub_formula, inst at 1 2, instantiate_formula, inst_formula.
-      f_equal; eapply inst_subst.
-    - unfold subst, sub_formula, inst at 1 2, instantiate_formula, inst_formula.
-      f_equal; eapply inst_subst.
-    - unfold subst, sub_formula, inst at 1 2, instantiate_formula, inst_formula.
-      repeat f_equal; eapply inst_subst.
+    constructor; auto. intros Σ Σ' ζ ι t.
+    induction t; cbn; repeat f_equal; apply inst_subst.
   Qed.
 
   Global Instance OccursCheckFormula : OccursCheck Formula :=
@@ -193,63 +173,17 @@ Module Assertions
   Global Instance OccursCheckLawsFormula : OccursCheckLaws Formula.
   Proof.
     constructor.
-    - intros ? ? ? ? []; cbn;
-        now rewrite ?occurs_check_shift.
-    - intros ? ? ? [] fml' Heq; cbn in *.
-      + apply option_map_eq_some' in Heq; destruct_conjs; subst; cbn.
-        f_equal. apply (occurs_check_sound _ _ H).
-      + apply option_map_eq_some' in Heq; destruct_conjs; subst; cbn.
-        f_equal. now apply (occurs_check_sound (T := fun Σ => Term Σ _)).
-      + apply option_map_eq_some' in Heq; destruct_conjs; subst; cbn.
-        f_equal. now apply occurs_check_sound.
-      + apply option_bind_eq_some in Heq; destruct Heq as (f & Heq1 & Heq2).
-        apply option_bind_eq_some in Heq1; destruct Heq1 as (t1' & Heq11 & Heq12).
-        apply (occurs_check_sound (T := fun Σ => Term Σ _)) in Heq11. subst t1.
-        apply noConfusion_inv in Heq12; cbn in Heq12; subst f; cbn.
-        apply option_bind_eq_some in Heq2; destruct Heq2 as (t2' & Heq21 & Heq22).
-        apply (occurs_check_sound (T := fun Σ => Term Σ _)) in Heq21. subst t2.
-        apply noConfusion_inv in Heq22; cbn in Heq22; subst fml'; cbn.
-        reflexivity.
-      + apply option_bind_eq_some in Heq; destruct Heq as (f & Heq1 & Heq2).
-        apply option_bind_eq_some in Heq1; destruct Heq1 as (t1' & Heq11 & Heq12).
-        apply (occurs_check_sound (T := fun Σ => Term Σ _)) in Heq11. subst t1.
-        apply noConfusion_inv in Heq12; cbn in Heq12; subst f; cbn.
-        apply option_bind_eq_some in Heq2; destruct Heq2 as (t2' & Heq21 & Heq22).
-        apply (occurs_check_sound (T := fun Σ => Term Σ _)) in Heq21. subst t2.
-        apply noConfusion_inv in Heq22; cbn in Heq22; subst fml'; cbn.
-        reflexivity.
-      + apply option_bind_eq_some in Heq; destruct Heq as (f & Heq1 & Heq2).
-        apply option_bind_eq_some in Heq1; destruct Heq1 as (t1' & Heq11 & Heq12).
-        apply (occurs_check_sound (T := fun Σ => Term Σ _)) in Heq11. subst t1.
-        apply noConfusion_inv in Heq12; cbn in Heq12; subst f; cbn.
-        apply option_bind_eq_some in Heq2; destruct Heq2 as (t2' & Heq21 & Heq22).
-        apply (occurs_check_sound (T := fun Σ => Term Σ _)) in Heq21. subst t2.
-        apply noConfusion_inv in Heq22; cbn in Heq22; subst fml'; cbn.
-        reflexivity.
-      + apply option_bind_eq_some in Heq; destruct Heq as (f & Heq1 & Heq2).
-        apply option_bind_eq_some in Heq1; destruct Heq1 as (t1' & Heq11 & Heq12).
-        apply (occurs_check_sound (T := fun Σ => Term Σ _)) in Heq11. subst t1.
-        apply noConfusion_inv in Heq12; cbn in Heq12; subst f; cbn.
-        apply option_bind_eq_some in Heq2; destruct Heq2 as (t2' & Heq21 & Heq22).
-        apply (occurs_check_sound (T := fun Σ => Term Σ _)) in Heq21. subst t2.
-        apply noConfusion_inv in Heq22; cbn in Heq22; subst fml'; cbn.
-        reflexivity.
-      + apply option_bind_eq_some in Heq; destruct Heq as (f & Heq1 & Heq2).
-        apply option_bind_eq_some in Heq1; destruct Heq1 as (t1' & Heq11 & Heq12).
-        apply (occurs_check_sound (T := fun Σ => Term Σ _)) in Heq11. subst t1.
-        apply noConfusion_inv in Heq12; cbn in Heq12; subst f; cbn.
-        apply option_bind_eq_some in Heq2; destruct Heq2 as (t2' & Heq21 & Heq22).
-        apply (occurs_check_sound (T := fun Σ => Term Σ _)) in Heq21. subst t2.
-        apply noConfusion_inv in Heq22; cbn in Heq22; subst fml'; cbn.
-        reflexivity.
-      + apply option_bind_eq_some in Heq; destruct Heq as (f & Heq1 & Heq2).
-        apply option_bind_eq_some in Heq1; destruct Heq1 as (t1' & Heq11 & Heq12).
-        apply (occurs_check_sound (T := fun Σ => Term Σ _)) in Heq11. subst t1.
-        apply noConfusion_inv in Heq12; cbn in Heq12; subst f; cbn.
-        apply option_bind_eq_some in Heq2; destruct Heq2 as (t2' & Heq21 & Heq22).
-        apply (occurs_check_sound (T := fun Σ => Term Σ _)) in Heq21. subst t2.
-        apply noConfusion_inv in Heq22; cbn in Heq22; subst fml'; cbn.
-        reflexivity.
+    - intros ? ? ? ? []; cbn; now rewrite ?occurs_check_shift.
+    - intros ? ? ? [] fml' Heq; cbn in *;
+        repeat
+          lazymatch goal with
+          | H: option_map _ _ = Some _ |- _ =>
+              apply option_map_eq_some' in H; destruct_conjs; subst; cbn
+          | H: option_ap _ _ = Some _ |- _ =>
+              apply option_bind_eq_some in H; destruct_conjs; subst; cbn
+          | H: @occurs_check ?T ?OC ?Σ ?b ?bIn ?t = Some ?t' |- _ =>
+              apply (@occurs_check_sound T _ OC _ Σ b bIn t t') in H; subst
+          end; auto.
   Qed.
 
   (* The path condition expresses a set of constraints on the logic variables
@@ -768,6 +702,1109 @@ Module Assertions
 
   End Messages.
 
+  Section Worlds.
+
+    Record World : Type :=
+      MkWorld
+        { wctx :> LCtx;
+          wco  : PathCondition wctx;
+        }.
+
+    Definition wnil : World := @MkWorld ctx_nil nil.
+    Definition wsnoc (w : World) (b : 𝑺 * Ty) : World :=
+      @MkWorld (wctx w ▻ b) (subst (wco w) sub_wk1).
+    Definition wformula (w : World) (f : Formula w) : World :=
+      @MkWorld (wctx w) (cons f (wco w)).
+    Definition wsubst (w : World) x {σ} {xIn : x :: σ ∈ w} (t : Term (w - (x :: σ)) σ) : World :=
+      {| wctx := wctx w - (x :: σ); wco := subst (wco w) (sub_single xIn t) |}.
+    Global Arguments wsubst w x {σ xIn} t.
+    Definition wcat (w : World) (Δ : LCtx) : World :=
+      @MkWorld (wctx w ▻▻ Δ) (subst (wco w) (sub_cat_left Δ)).
+    Definition wformulas (w : World) (fmls : List Formula w) : World :=
+      @MkWorld (wctx w) (app fmls (wco w)).
+
+    Definition TYPE : Type := World -> Type.
+    Bind Scope modal with TYPE.
+    Definition Valid (A : TYPE) : Type :=
+      forall w, A w.
+    Definition Impl (A B : TYPE) : TYPE :=
+      fun w => A w -> B w.
+    Definition Forall {I : Type} (A : I -> TYPE) : TYPE :=
+      fun w => forall i : I, A i w.
+    (* Definition Cat (A : TYPE) (Δ : LCtx) : TYPE := *)
+    (*   fun w => A (wcat w Δ). *)
+
+  End Worlds.
+
+  Section TriangularSubstitutions.
+
+    Ltac rew := rewrite ?subst_sub_comp, ?subst_shift_single, ?subst_sub_id, ?sub_comp_id_right,
+        ?sub_comp_id_left, ?inst_sub_id, ?inst_sub_id.
+
+    Inductive Tri (w : World) : World -> Type :=
+    | tri_id        : Tri w w
+    | tri_cons {w' x σ}
+        (xIn : (x::σ) ∈ w) (t : Term (wctx w - (x::σ)) σ)
+        (ν : Tri (wsubst w x t) w') : Tri w w'.
+    Global Arguments tri_id {_}.
+    Global Arguments tri_cons {_ _} x {_ _} t ν.
+
+    Fixpoint tri_comp {w1 w2 w3} (ν12 : Tri w1 w2) : Tri w2 w3 -> Tri w1 w3 :=
+      match ν12 with
+      | tri_id           => fun ν => ν
+      | tri_cons x t ν12 => fun ν => tri_cons x t (tri_comp ν12 ν)
+      end.
+
+    Fixpoint sub_triangular {w1 w2} (ζ : Tri w1 w2) : Sub w1 w2 :=
+      match ζ with
+      | tri_id         => sub_id _
+      | tri_cons x t ζ => subst (sub_single _ t) (sub_triangular ζ)
+      end.
+
+    Lemma sub_triangular_comp {w0 w1 w2} (ν01 : Tri w0 w1) (ν12 : Tri w1 w2) :
+      sub_triangular (tri_comp ν01 ν12) =
+      subst (sub_triangular ν01) (sub_triangular ν12).
+    Proof.
+      induction ν01; cbn [sub_triangular tri_comp].
+      - now rew.
+      - now rewrite sub_comp_assoc, IHν01.
+    Qed.
+
+    Fixpoint sub_triangular_inv {w1 w2} (ζ : Tri w1 w2) : Sub w2 w1 :=
+      match ζ with
+      | tri_id         => sub_id _
+      | tri_cons x t ζ => subst (sub_triangular_inv ζ) (sub_shift _)
+      end.
+
+    Lemma sub_triangular_inv_comp {w0 w1 w2} (ν01 : Tri w0 w1) (ν12 : Tri w1 w2) :
+      sub_triangular_inv (tri_comp ν01 ν12) =
+      subst (sub_triangular_inv ν12) (sub_triangular_inv ν01).
+    Proof.
+      induction ν01; cbn.
+      - now rew.
+      - now rewrite IHν01, sub_comp_assoc.
+    Qed.
+
+    Fixpoint inst_triangular {w0 w1} (ζ : Tri w0 w1) (ι : SymInstance w0) : Prop :=
+      match ζ with
+      | tri_id => True
+      | @tri_cons _ Σ' x σ xIn t ζ0 =>
+        let ι' := env_remove (x :: σ) ι xIn in
+        env_lookup ι xIn = inst t ι' /\ inst_triangular ζ0 ι'
+      end.
+
+    Lemma inst_triangular_left_inverse {w1 w2 : World} (ι2 : SymInstance w2) (ν : Tri w1 w2) :
+      inst (sub_triangular_inv ν) (inst (sub_triangular ν) ι2) = ι2.
+    Proof. rewrite <- inst_subst. induction ν; cbn - [subst]; now rew. Qed.
+
+    Lemma inst_triangular_right_inverse {w1 w2 : World} (ι1 : SymInstance w1) (ζ : Tri w1 w2) :
+      inst_triangular ζ ι1 ->
+      inst (sub_triangular ζ) (inst (sub_triangular_inv ζ) ι1) = ι1.
+    Proof.
+      intros Hζ. induction ζ; cbn - [subst].
+      - now rew.
+      - cbn in Hζ. rewrite <- inst_sub_shift in Hζ. destruct Hζ as [? Hζ].
+        rewrite ?inst_subst, IHζ, inst_sub_single_shift; auto.
+    Qed.
+
+    (* Forward entailment *)
+    Lemma entails_triangular_inv {w0 w1} (ν : Tri w0 w1) (ι0 : SymInstance w0) :
+      inst_triangular ν ι0 ->
+      instpc (wco w0) ι0 ->
+      instpc (wco w1) (inst (sub_triangular_inv ν) ι0).
+    Proof.
+      induction ν; cbn.
+      - cbn. rewrite inst_sub_id. auto.
+      - rewrite <- inst_sub_shift, inst_subst. intros [Heqx Heq'] Hpc0.
+        apply IHν; cbn; auto.
+        rewrite inst_subst, inst_sub_single_shift; auto.
+    Qed.
+
+    Lemma inst_triangular_valid {w0 w1} (ζ01 : Tri w0 w1) (ι1 : SymInstance w1) :
+      inst_triangular ζ01 (inst (sub_triangular ζ01) ι1).
+    Proof.
+      induction ζ01; cbn; auto.
+      rewrite <- inst_lookup, lookup_sub_comp. rewrite lookup_sub_single_eq.
+      rewrite <- inst_sub_shift. rewrite <- ?inst_subst.
+      rewrite subst_sub_comp.
+      rewrite subst_shift_single.
+      split; auto.
+      rewrite <- ?sub_comp_assoc.
+      rewrite sub_comp_shift_single.
+      rewrite sub_comp_id_left.
+      auto.
+    Qed.
+
+    Lemma inst_tri_comp {w0 w1 w2} (ν01 : Tri w0 w1) (ν12 : Tri w1 w2) (ι0 : SymInstance w0) :
+      inst_triangular (tri_comp ν01 ν12) ι0 <->
+      inst_triangular ν01 ι0 /\ inst_triangular ν12 (inst (sub_triangular_inv ν01) ι0).
+    Proof.
+      induction ν01; cbn.
+      - rewrite inst_sub_id; intuition.
+      - rewrite ?inst_subst, ?inst_sub_shift. split.
+        + intros (Heq & Hwp). apply IHν01 in Hwp. now destruct Hwp.
+        + intros ([Heq Hν01] & Hwp). split; auto. apply IHν01; auto.
+    Qed.
+
+  End TriangularSubstitutions.
+
+  Section Accessibility.
+
+    Import Entailment.
+
+    Inductive Acc (w1 : World) : World -> Type :=
+    | acc_refl : Acc w1 w1
+    | acc_sub {w2 : World} (ζ : Sub w1 w2) (ent : wco w2 ⊢ subst (wco w1) ζ) : Acc w1 w2.
+    Global Arguments acc_refl {w} : rename.
+    Global Arguments acc_sub {w1 w2} ζ ent.
+    Notation "w1 ⊒ w2" := (Acc w1 w2) (at level 80).
+
+    Equations(noeqns) acc_trans {w0 w1 w2} (ω01 : w0 ⊒ w1) (ω12 : w1 ⊒ w2) : w0 ⊒ w2 :=
+    | acc_refl         | ω12              := ω12;
+    | ω01              | acc_refl         := ω01;
+    | acc_sub ζ01 ent1 | acc_sub ζ12 ent2 := acc_sub (subst (T := Sub _) ζ01 ζ12) _.
+    Next Obligation.
+      intros w0 w1 w2 ζ01 Hpc01 ζ12 Hpc12. transitivity (subst (wco w1) ζ12); auto.
+      rewrite subst_sub_comp. now apply proper_subst_entails.
+    Qed.
+    Global Arguments acc_trans {w0 w1 w2} !ω01 !ω12.
+
+    Definition sub_acc {w1 w2} (ω : w1 ⊒ w2) : Sub (wctx w1) (wctx w2) :=
+      match ω with
+      | acc_refl    => sub_id _
+      | acc_sub ζ _ => ζ
+      end.
+
+    Lemma sub_acc_trans {w0 w1 w2} (ω01 : w0 ⊒ w1) (ω12 : w1 ⊒ w2) :
+      sub_acc (acc_trans ω01 ω12) = subst (sub_acc ω01) (sub_acc ω12).
+    Proof.
+      destruct ω01, ω12; cbn - [subst];
+        now rewrite ?sub_comp_id_left, ?sub_comp_id_right.
+    Qed.
+
+    Definition Box (A : TYPE) : TYPE :=
+      fun w0 => forall w1, w0 ⊒ w1 -> A w1.
+
+    Lemma ent_acc_sub {w1 w2} (ω : w1 ⊒ w2) :
+      wco w2 ⊢ subst (wco w1) (sub_acc ω).
+    Proof. destruct ω; cbn; now rewrite ?subst_sub_id. Qed.
+
+    Definition acc_snoc_right {w} {b : 𝑺 * Ty} : w ⊒ wsnoc w b :=
+      @acc_sub w (wsnoc w b) sub_wk1 (entails_refl (subst (wco w) sub_wk1)).
+
+    Program Definition acc_snoc_left {w1 w2} (ω12 : w1 ⊒ w2) (b : 𝑺 * Ty) (t : Term w2 (snd b)) :
+      wsnoc w1 b ⊒ w2 := acc_sub (sub_snoc (sub_acc ω12) b t) _.
+    Next Obligation.
+    Proof.
+      intros *. unfold wsnoc. cbn [wctx wco].
+      rewrite subst_wk1_snoc.
+      apply ent_acc_sub.
+    Qed.
+
+    Definition acc_snoc_left' {w : World} b (t : Term w (snd b)) :
+      wsnoc w b ⊒ w := acc_snoc_left acc_refl b t.
+
+    Program Definition acc_cat_left {w1 w2} (ω12 : w1 ⊒ w2) {Δ : LCtx} (ζ : Sub Δ w2) :
+      wcat w1 Δ ⊒ w2 := acc_sub (sub_acc ω12 ►► ζ) _.
+    Next Obligation.
+    Proof.
+      intros *. unfold wcat. cbn [wctx wco].
+      rewrite <- subst_sub_comp.
+      rewrite sub_comp_cat_left.
+      apply ent_acc_sub.
+    Qed.
+
+    Program Definition acc_formula_right {w : World} (f : Formula w) : w ⊒ wformula w f :=
+      @acc_sub w (wformula w f) (sub_id (wctx w)) _.
+    Next Obligation.
+    Proof.
+      intros * ι. unfold wformula. cbn.
+      rewrite subst_sub_id.
+      rewrite inst_pathcondition_cons.
+      now intros [].
+    Qed.
+
+    Program Definition acc_formulas_right (w : World) (fmls : List Formula w) :
+      w ⊒ wformulas w fmls :=
+      @acc_sub w (wformulas w fmls) (sub_id (wctx w)) _.
+    Next Obligation.
+    Proof.
+      intros w fmls ι. cbn.
+      rewrite subst_sub_id.
+      rewrite inst_pathcondition_app.
+      now intros [].
+    Qed.
+
+    Definition acc_subst_right {w : World} x {σ} {xIn : x :: σ ∈ w} (t : Term (w - (x :: σ)) σ) :
+      w ⊒ wsubst w x t :=
+      let ζ  := sub_single xIn t in
+      let w' := {| wctx := w - (x :: σ); wco := subst (wco w) ζ |}  in
+      @acc_sub w w' ζ (entails_refl (wco w')).
+    Arguments acc_subst_right {w} x {σ xIn} t.
+
+    Fixpoint acc_triangular {w1 w2} (ν : Tri w1 w2) : w1 ⊒ w2 :=
+      match ν with
+      | tri_id         => acc_refl
+      | tri_cons x t ν => acc_trans (acc_subst_right x t) (acc_triangular ν)
+      end.
+
+    Lemma sub_acc_triangular {w1 w2} (ζ : Tri w1 w2) :
+      sub_acc (acc_triangular ζ) = sub_triangular ζ.
+    Proof.
+      induction ζ; cbn.
+      - reflexivity.
+      - now rewrite sub_acc_trans, IHζ.
+    Qed.
+
+    (* Lemma acc_triangular_app {w0 w1 w2} (ν01 : Tri w0 w1) (ν12 : Tri w1 w2) : *)
+    (*   wsub (acc_triangular (tri_comp ν01 ν12)) = *)
+    (*   subst (sub_acc (acc_triangular ν01)) (sub_acc (acc_triangular ν12)). *)
+    (* Proof. *)
+    (*   induction ν01; cbn - [SubstEnv]. *)
+    (*   - now rewrite sub_comp_id_left. *)
+    (*   - rewrite <- subst_sub_comp. now f_equal. *)
+    (* Qed. *)
+
+  End Accessibility.
+
+  Instance preorder_acc : CRelationClasses.PreOrder Acc :=
+    CRelationClasses.Build_PreOrder Acc (@acc_refl) (@acc_trans).
+
+  Declare Scope modal.
+  Delimit Scope modal with modal.
+
+  Section S4.
+
+    Notation "⊢ A" := (Valid A%modal) (at level 100).
+    Notation "A -> B" := (Impl A%modal B%modal) : modal.
+    Notation "□ A" := (Box A%modal) (at level 9, format "□ A", right associativity) : modal.
+
+    Definition K {A B} :
+      ⊢ □(A -> B) -> (□A -> □B) :=
+      fun w0 f a w1 ω01 =>
+        f w1 ω01 (a w1 ω01).
+    Definition T {A} :
+      ⊢ □A -> A :=
+      fun w0 a => a w0 acc_refl.
+    Definition four {A} :
+      ⊢ □A -> □□A :=
+      fun w0 a w1 ω01 w2 ω12 =>
+        a w2 (acc_trans ω01 ω12).
+    Global Arguments four : simpl never.
+
+    (* faster version of (four _ sub_wk1) *)
+    (* Definition four_wk1 {A} : *)
+    (*   ⊢ □A -> ∀ b, Snoc (□A) b := *)
+    (*   fun w0 a b w1 ω01 => a w1 (env_tail ω01). *)
+    (* Arguments four_wk1 {A Σ0} pc0 a b [Σ1] ζ01 : rename. *)
+
+    Definition fmap_box {A B} (f : ⊢ A -> B) : ⊢ □A -> □B :=
+      fun w0 a w1 ω01 => f w1 (a w1 ω01).
+    Definition extend_box {A B} (f : ⊢ □A -> B) : ⊢ □A -> □B :=
+      fun w0 a w1 ω01 => f w1 (four a ω01).
+    Definition comp {A B C} :
+      ⊢ (B -> C) -> (A -> B) -> (A -> C) :=
+      fun w0 => Basics.compose.
+
+  End S4.
+
+  Module ModalNotations.
+
+    Notation "⊢ A" := (Valid A%modal) (at level 100).
+    Notation "A -> B" := (Impl A%modal B%modal) : modal.
+    Notation "□ A" := (Box A%modal) (at level 9, format "□ A", right associativity) : modal.
+    Notation "⌜ A ⌝" := (fun (w : World) => Const A%type w) (at level 0, format "⌜ A ⌝") : modal.
+    Notation "'∀' x .. y , P " :=
+      (Forall (fun x => .. (Forall (fun y => P%modal)) ..))
+        (at level 99, x binder, y binder, right associativity)
+      : modal.
+    Notation "w1 ⊒ w2" := (Acc w1 w2) (at level 80).
+    Notation "f <$> a" := (fmap_box f a) (at level 40, left associativity).
+    Notation "f <*> a" := (K f a) (at level 40, left associativity).
+
+  End ModalNotations.
+  Open Scope modal.
+
+  Section Persistence.
+
+    Import Entailment.
+    Import ModalNotations.
+
+    Class Persistent (A : TYPE) (* `{LogicalRelation.LR A} *) : Type :=
+      persist     : ⊢ A -> □A.
+        (* persist_lr  : forall w0 (a : A w0) w1 (ω01 : w0 ⊒ w1), *)
+        (*     LogicalRelation.lr ω01 a (persist a ω01); *)
+        (* persist_dcl : *)
+        (*   forall w (a : A w), *)
+        (*     LogicalRelation.dcl (persist a) *)
+    (* Global Arguments Persistent A {_}. *)
+
+    Global Instance persistent_subst {A} `{Subst A} : Persistent A :=
+      fun w0 x w1 ω01 =>
+        match ω01 with
+        | acc_refl => x
+        | @acc_sub _ w2 ζ _ => subst x ζ
+        end.
+
+    Lemma persist_subst {A} `{SubstLaws A} {w1 w2} {ω : w1 ⊒ w2} {a : A w1} :
+      persist a ω = subst a (sub_acc ω).
+    Proof. destruct ω; cbn; now rewrite ?subst_sub_id. Qed.
+
+    Lemma persist_trans {A} `{SubstLaws A} {w0 w1 w2} {ω1 : w0 ⊒ w1} {ω2 : w1 ⊒ w2} {a : A w0} :
+      persist a (acc_trans ω1 ω2) = persist (persist a ω1) ω2.
+    Proof. now rewrite ?persist_subst, sub_acc_trans, subst_sub_comp. Qed.
+
+    Lemma inst_persist  {AT A} `{InstLaws AT A} {w1 w2} (ω : w1 ⊒ w2) :
+      forall (ι : SymInstance w2) (t : AT w1),
+        inst (persist t ω) ι = inst t (inst (sub_acc ω) ι).
+    Proof. intros. now rewrite persist_subst, inst_subst. Qed.
+
+    Lemma ent_acc {w1 w2} (ω : w1 ⊒ w2) :
+      wco w2 ⊢ persist (wco w1) ω.
+    Proof. destruct ω; cbn; now rewrite ?subst_sub_id. Qed.
+
+    (* Program Definition acc_snoc {w0 w1} (ω01 : w0 ⊒ w1) (b : 𝑺 * Ty) : *)
+    (*   wsnoc w0 b ⊒ wsnoc w1 b := *)
+    (*   match ω01 in _ ⊒ w return wsnoc w0 b ⊒ wsnoc w b with *)
+    (*   | acc_refl            => acc_refl *)
+    (*   | @acc_sub _ w2 ζ ent => @acc_sub _ (wsnoc _ b) (sub_up1 ζ) _ *)
+    (*   end. *)
+    (* Next Obligation. *)
+    (* Proof. *)
+    (*   intros. unfold wsnoc; cbn. *)
+    (*   rewrite <- subst_sub_comp. *)
+    (*   rewrite sub_comp_wk1_comm. *)
+    (*   rewrite subst_sub_comp. *)
+    (*   now apply proper_subst_entails. *)
+    (* Qed. *)
+
+    (* Program Definition acc_formula {w0 w1} (ω01 : w0 ⊒ w1) (fml : Formula w0) : *)
+    (*   wformula w0 fml ⊒ wformula w1 (persist fml ω01) := *)
+    (*   @acc_sub (MkWorld (cons fml (wco w0))) (MkWorld (cons (persist fml ω01) (wco w1))) (sub_acc ω01) _. *)
+    (* Next Obligation. *)
+    (*   intros ? ? ? ? ι. *)
+    (*   unfold wformula in *. *)
+    (*   cbn [wco wctx] in *. cbn. *)
+    (*   destruct ω01; cbn. *)
+    (*   - now rewrite ?subst_sub_id. *)
+    (*   - rewrite ?inst_pathcondition_cons. *)
+    (*     intuition. *)
+    (* Qed. *)
+
+  End Persistence.
+
+  Notation WList A := (fun w : World => list (A w)).
+  Notation WTerm σ := (fun w : World => Term (wctx w) σ).
+  Notation STerm σ := (fun Σ => Term Σ σ).
+
+  Notation persist__term t :=
+    (@persist (WTerm _) (@persistent_subst (STerm _) (@SubstTerm _)) _ t).
+
+  Definition Solver : Type :=
+    forall w0 (fmls0 : WList Formula w0),
+      option { w1 & Tri w0 w1 * List Formula w1 }%type.
+
+  Definition SolverSpec (s : Solver) : Prop :=
+    forall w0 (fmls0 : WList Formula w0),
+      OptionSpec
+        (fun '(existT w1 (ζ, fmls1)) =>
+           forall ι0,
+             instpc (wco w0) ι0 ->
+             (instpc fmls0 ι0 -> inst_triangular ζ ι0) /\
+               (forall ι1,
+                   instpc (wco w1) ι1 ->
+                   ι0 = inst (sub_triangular ζ) ι1 ->
+                   instpc fmls0 ι0 <-> inst fmls1 ι1))
+        (forall ι, instpc (wco w0) ι -> ~ instpc fmls0 ι)
+        (s w0 fmls0).
+
+  Definition SoundSolver : Type :=
+    { s : Solver | SolverSpec s }.
+
+  Module Solver.
+
+    Equations(noeqns) simplify_formula_bool_binop {Σ σ1 σ2} (op : BinOp σ1 σ2 ty_bool) (t1 : STerm σ1 Σ) (t2 : STerm σ2 Σ) (k : List Formula Σ) : List Formula Σ :=
+    | binop_eq  | t1 | t2 | k := cons (formula_eq t1 t2) k;
+    | binop_le  | t1 | t2 | k := cons (formula_le t1 t2) k;
+    | binop_lt  | t1 | t2 | k := cons (formula_lt t1 t2) k;
+    | binop_ge  | t1 | t2 | k := cons (formula_ge t1 t2) k;
+    | binop_gt  | t1 | t2 | k := cons (formula_gt t1 t2) k;
+    | binop_and | t1 | t2 | k := cons (formula_bool t1) (cons (formula_bool t2) k);
+    | op        | t1 | t2 | k := cons (formula_bool (term_binop op t1 t2)) k.
+
+    Equations(noeqns) simplify_formula_bool_binop_neg {Σ σ1 σ2} (op : BinOp σ1 σ2 ty_bool) (t1 : STerm σ1 Σ) (t2 : STerm σ2 Σ) (k : List Formula Σ) : List Formula Σ :=
+    | binop_eq  | t1 | t2 | k := cons (formula_neq t1 t2) k;
+    | binop_le  | t1 | t2 | k := cons (formula_gt t1 t2) k;
+    | binop_lt  | t1 | t2 | k := cons (formula_ge t1 t2) k;
+    | binop_ge  | t1 | t2 | k := cons (formula_lt t1 t2) k;
+    | binop_gt  | t1 | t2 | k := cons (formula_le t1 t2) k;
+    | binop_or  | t1 | t2 | k := cons (formula_bool (term_not t1)) (cons (formula_bool (term_not t2)) k);
+    | op        | t1 | t2 | k := cons (formula_bool (term_not (term_binop op t1 t2))) k.
+
+    Lemma simplify_formula_bool_binop_spec {Σ σ1 σ2} (op : BinOp σ1 σ2 ty_bool) t1 t2 (k : List Formula Σ) :
+      forall ι : SymInstance Σ,
+        instpc (simplify_formula_bool_binop op t1 t2 k) ι <->
+          eval_binop op (inst t1 ι) (inst t2 ι) = true /\ instpc k ι.
+    Proof.
+      intros; dependent elimination op; cbn;
+        rewrite ?inst_pathcondition_cons, ?andb_true_iff; cbn;
+        rewrite ?Z.eqb_eq, ?Z.leb_le, ?Z.ltb_lt, ?Z.geb_le, ?Z.ge_le_iff,
+          ?Z.gtb_lt, ?Z.gt_lt_iff, ?and_assoc;
+        try reflexivity.
+    Qed.
+
+    Lemma simplify_formula_bool_binop_neg_spec {Σ σ1 σ2} (op : BinOp σ1 σ2 ty_bool) t1 t2 k :
+      forall ι : SymInstance Σ,
+        instpc (simplify_formula_bool_binop_neg op t1 t2 k) ι <->
+          eval_binop op (inst t1 ι) (inst t2 ι) = false /\ instpc k ι.
+    Proof.
+      intros; dependent elimination op; cbn;
+        rewrite ?inst_pathcondition_cons; cbn;
+        change (inst_term ?t ?ι) with (inst t ι);
+        rewrite ?Z.eqb_neq, ?Z.leb_gt, ?Z.gt_lt_iff, ?Z.ltb_ge, ?Z.ge_le_iff,
+          ?Z.geb_leb, ?Z.leb_gt, ?Z.gtb_ltb, ?Z.ltb_ge,
+          ?orb_false_iff, ?negb_true_iff, ?and_assoc;
+        reflexivity.
+    Qed.
+
+    Equations(noeqns) simplify_formula_bool {Σ} (t : Term Σ ty_bool) (k : List Formula Σ) : option (List Formula Σ) :=
+    | term_var ς                 | k := Some (cons (formula_bool (term_var ς)) k);
+    | term_lit _ b               | k := if b then Some k else None;
+    | term_binop op t1 t2        | k := Some (simplify_formula_bool_binop op t1 t2 k);
+    | term_not t                 | k := simplify_formula_bool_neg t k;
+    | @term_projtup _ _ t n _ p  | k := Some (cons (formula_bool (@term_projtup _ _ t n _ p)) k)
+    with simplify_formula_bool_neg {Σ} (t : Term Σ ty_bool) (k : List Formula Σ) : option (List Formula Σ) :=
+    | term_var ς                | k := Some (cons (formula_bool (term_not (term_var ς))) k);
+    | term_lit _ b              | k := if b then None else Some k;
+    | term_binop op t1 t2        | k := Some (simplify_formula_bool_binop_neg op t1 t2 k);
+    | term_not t                | k := simplify_formula_bool t k;
+    | @term_projtup _ _ t n _ p | k := Some (cons (formula_bool (term_not (@term_projtup _ _ t n _ p))) k).
+
+    Definition simplify_formula_eqb {Σ σ} (t1 t2 : Term Σ σ) (k : List Formula Σ) : option (List Formula Σ) :=
+      if Term_eqb t1 t2
+      then Some k
+      else Some (cons (formula_eq t1 t2) k).
+
+    Lemma simplify_formula_eqb_spec {Σ σ} (t1 t2 : Term Σ σ) (k : List Formula Σ) :
+      OptionSpec
+        (fun fmlsk => forall ι, instpc fmlsk ι <-> inst (formula_eq t1 t2) ι /\ instpc k ι)
+        (forall ι, ~ inst (formula_eq t1 t2) ι)
+        (simplify_formula_eqb t1 t2 k).
+    Proof.
+      unfold simplify_formula_eqb.
+      destruct (Term_eqb_spec t1 t2); constructor; intros ι.
+      - subst; intuition.
+      - now rewrite inst_pathcondition_cons.
+    Qed.
+
+    Equations(noeqns) simplify_formula_eq_binop {Σ σ σ11 σ12 σ21 σ22}
+      (op1 : BinOp σ11 σ12 σ) (t11 : Term Σ σ11) (t12 : Term Σ σ12)
+      (op2 : BinOp σ21 σ22 σ) (t21 : Term Σ σ21) (t22 : Term Σ σ22)
+      (k : List Formula Σ) : option (List Formula Σ) :=
+    | binop_pair | t11 | t12 | binop_pair | t21 | t22 | k :=
+      Some (cons (formula_eq t11 t21) (cons (formula_eq t12 t22) k));
+    | binop_cons | t11 | t12 | binop_cons | t21 | t22 | k :=
+      Some (cons (formula_eq t11 t21) (cons (formula_eq t12 t22) k));
+    | op1        | t11 | t12 | op2        | t21 | t22 | k :=
+      simplify_formula_eqb (term_binop op1 t11 t12) (term_binop op2 t21 t22) k.
+
+    Lemma simplify_formula_eq_binop_spec {Σ σ σ11 σ12 σ21 σ22}
+      (op1 : BinOp σ11 σ12 σ) (t11 : Term Σ σ11) (t12 : Term Σ σ12)
+      (op2 : BinOp σ21 σ22 σ) (t21 : Term Σ σ21) (t22 : Term Σ σ22)
+      (k : List Formula Σ) :
+      OptionSpec
+        (fun fmlsk : List Formula Σ =>
+           forall ι,
+             instpc fmlsk ι <->
+               eval_binop op1 (inst t11 ι) (inst t12 ι) =
+               eval_binop op2 (inst t21 ι) (inst t22 ι) /\ instpc k ι)
+        (forall ι, eval_binop op1 (inst t11 ι) (inst t12 ι) <>
+                   eval_binop op2 (inst t21 ι) (inst t22 ι))
+        (simplify_formula_eq_binop op1 t11 t12 op2 t21 t22 k).
+    Proof.
+      destruct op1; cbn;
+        try match goal with
+            | |- OptionSpec _ _ (simplify_formula_eqb ?t1 ?t2 ?k) =>
+                generalize (simplify_formula_eqb_spec t1 t2 k);
+                let H := fresh in
+                let ι := fresh "ι" in
+                apply optionspec_monotonic;
+                [ let pc := fresh "pc" in intros pc |];
+                intros H ι; specialize (H ι); auto
+                (* change (inst_term ?t ?ι) with (inst t ι); auto *)
+            end.
+      - dependent elimination op2; cbn. constructor. intros ι.
+        rewrite ?inst_pathcondition_cons. cbn. intuition.
+      - dependent elimination op2; cbn.
+        + constructor. intros ι.
+          rewrite ?inst_pathcondition_cons. cbn. intuition.
+        + constructor. intros ι.
+          rewrite ?inst_pathcondition_cons. cbn. intuition.
+    Qed.
+
+    Equations(noeqns) simplify_formula_eq_binop_lit {Σ σ σ1 σ2}
+      (op : BinOp σ1 σ2 σ) (t1 : Term Σ σ1) (t2 : Term Σ σ2) (v : Lit σ)
+      (k : List Formula Σ) : option (List Formula Σ) :=
+    | binop_pair | t1 | t2 | (v1 , v2) | k :=
+      Some (cons (formula_eq t1 (term_lit _ v1)) (cons (formula_eq t2 (term_lit _ v2)) k));
+    | binop_cons | t1 | t2 | nil | k := None;
+    | binop_cons | t1 | t2 | cons v1 v2 | k :=
+      Some (cons (formula_eq t1 (term_lit _ v1)) (cons (formula_eq t2 (term_lit (ty_list _) v2)) k));
+    | op         | t1 | t2 | v         | k :=
+      Some (cons (formula_eq (term_binop op t1 t2) (term_lit _ v)) k).
+
+    Lemma simplify_formula_eq_binop_lit_spec {Σ σ σ1 σ2}
+      (op : BinOp σ1 σ2 σ) (t1 : Term Σ σ1) (t2 : Term Σ σ2) (v : Lit σ) (k : List Formula Σ) :
+      OptionSpec
+        (fun fmlsk : List Formula Σ =>
+           forall ι, instpc fmlsk ι <-> eval_binop op (inst t1 ι) (inst t2 ι) = v /\ instpc k ι)
+        (forall ι, eval_binop op (inst t1 ι) (inst t2 ι) <> v)
+        (simplify_formula_eq_binop_lit op t1 t2 v k).
+    Proof.
+      destruct op; cbn; try (constructor; intros ι); cbn;
+        rewrite ?inst_pathcondition_cons; cbn; try reflexivity.
+      - destruct v. constructor. intros ι. cbn.
+        rewrite ?inst_pathcondition_cons. cbn. intuition.
+      - destruct v; constructor; intros ι; cbn.
+        + discriminate.
+        + rewrite ?inst_pathcondition_cons. cbn. intuition.
+    Qed.
+
+    Equations(noeqns) simplify_formula_eq {Σ σ} (t1 t2 : Term Σ σ) (k : List Formula Σ) : option (List Formula Σ) :=
+    | term_lit ?(σ) l1       | term_lit σ l2          | k => if Lit_eqb σ l1 l2 then Some k else None;
+    | term_inr _             | term_inl _             | k => None;
+    | term_inl _             | term_inr _             | k => None;
+    | term_inl t1            | term_inl t2            | k => simplify_formula_eq t1 t2 k;
+    | term_inr t1            | term_inr t2            | k => simplify_formula_eq t1 t2 k;
+    | term_record ?(R) ts1   | term_record R ts2      | k => Some (app (formula_eqs_nctx ts1 ts2) k);
+    | term_binop op1 t11 t12 | term_binop op2 t21 t22 | k => simplify_formula_eq_binop op1 t11 t12 op2 t21 t22 k;
+    | term_binop op1 t11 t12 | term_lit _ v           | k => simplify_formula_eq_binop_lit op1 t11 t12 v k;
+    | t1                     | t2                     | k => simplify_formula_eqb t1 t2 k.
+
+    Definition simplify_formula {Σ} (fml : Formula Σ) (k : List Formula Σ) : option (List Formula Σ) :=
+      match fml with
+      (* TODO: partial evaluation of ts *)
+      | formula_user p ts => Some (cons fml k)
+      | formula_bool t    => simplify_formula_bool (peval t) k
+      | formula_prop ζ P  => Some (cons fml k)
+      | formula_ge t1 t2  => simplify_formula_bool (peval (term_binop binop_ge t1 t2)) k
+      | formula_gt t1 t2  => simplify_formula_bool (peval (term_binop binop_gt t1 t2)) k
+      | formula_le t1 t2  => simplify_formula_bool (peval (term_binop binop_le t1 t2)) k
+      | formula_lt t1 t2  => simplify_formula_bool (peval (term_binop binop_lt t1 t2)) k
+      | formula_eq t1 t2  => simplify_formula_eq (peval t1) (peval t2) k
+      | formula_neq t1 t2 => Some (cons fml k)
+      end.
+
+    Fixpoint simplify_formulas {Σ} (fmls : List Formula Σ) (k : List Formula Σ) : option (List Formula Σ) :=
+      match fmls with
+      | nil           => Some k
+      | cons fml fmls =>
+        option_bind (simplify_formula fml) (simplify_formulas fmls k)
+      end.
+
+    Lemma simplify_formula_bool_spec {Σ} (t : Term Σ ty_bool) (k : List Formula Σ) :
+      OptionSpec
+        (fun fmlsk => forall ι, instpc fmlsk ι <-> inst (formula_bool t) ι /\ instpc k ι)
+        (forall ι, ~ inst (formula_bool t) ι)
+        (simplify_formula_bool t k)
+    with simplify_formula_bool_neg_spec {Σ} (t : Term Σ ty_bool) (k : List Formula Σ) :
+      OptionSpec
+        (fun fmlsk => forall ι, instpc fmlsk ι <-> ~ inst (formula_bool t) ι /\ instpc k ι)
+        (forall ι, inst (A := Prop) (formula_bool t) ι)
+        (simplify_formula_bool_neg t k).
+    Proof.
+      { dependent elimination t; cbn; try constructor.
+        - intros ι. rewrite inst_pathcondition_cons. reflexivity.
+        - destruct l; constructor; intuition.
+        - apply simplify_formula_bool_binop_spec.
+        - generalize (simplify_formula_bool_neg_spec Σ e0 k).
+          apply optionspec_monotonic.
+          + intros fmlsk HYP ι; specialize (HYP ι); revert HYP. cbn.
+            unfold is_true. now rewrite negb_true_iff, not_true_iff_false.
+          + intros HYP ι; specialize (HYP ι); revert HYP. cbn.
+            unfold is_true. now rewrite not_true_iff_false, negb_false_iff.
+        - intros ι. rewrite inst_pathcondition_cons. reflexivity.
+      }
+      { dependent elimination t; try constructor.
+        - intros ι. rewrite inst_pathcondition_cons. cbn.
+          unfold is_true. now rewrite negb_true_iff, not_true_iff_false.
+        - destruct l; cbn; constructor; intuition.
+        - intros ι. cbn. rewrite not_true_iff_false.
+          apply simplify_formula_bool_binop_neg_spec.
+        - generalize (simplify_formula_bool_spec Σ e0 k).
+          apply optionspec_monotonic.
+          + intros fmlsk HYP ι; specialize (HYP ι); revert HYP. cbn.
+            unfold is_true. now rewrite not_true_iff_false, negb_false_iff.
+          + intros HYP ι; specialize (HYP ι); revert HYP. cbn.
+            unfold is_true. now rewrite not_true_iff_false, negb_true_iff.
+        - intros ι. rewrite inst_pathcondition_cons. cbn.
+          unfold is_true. now rewrite negb_true_iff, not_true_iff_false.
+      }
+    Qed.
+
+    Lemma simplify_formula_eq_spec {Σ σ} (s t : Term Σ σ) (k : List Formula Σ) :
+      OptionSpec
+        (fun fmlsk : List Formula Σ => forall ι, instpc fmlsk ι <-> inst (formula_eq s t) ι /\ instpc k ι)
+        (forall ι, ~ inst (formula_eq s t) ι)
+        (simplify_formula_eq s t k).
+    Proof.
+      induction s; try apply simplify_formula_eqb_spec;
+        dependent elimination t; try (cbn; constructor; intros;
+          rewrite ?inst_pathcondition_cons; auto; fail).
+      - cbn. destruct (Lit_eqb_spec σ1 l l0); constructor; intuition.
+      - cbn. apply simplify_formula_eq_binop_lit_spec.
+      - cbn. apply simplify_formula_eq_binop_spec.
+      - specialize (IHs t). revert IHs. apply optionspec_monotonic.
+        + intros fmls HYP ι. specialize (HYP ι). rewrite HYP. cbn.
+          apply and_iff_compat_r. cbn. split; intros Heq.
+          * now f_equal.
+          * apply noConfusion_inv in Heq. apply Heq.
+        + intros HYP ι Heq. apply noConfusion_inv in Heq. apply (HYP ι Heq).
+      - specialize (IHs t0). revert IHs. apply optionspec_monotonic.
+        + intros fmls HYP ι. specialize (HYP ι). rewrite HYP. cbn.
+          apply and_iff_compat_r. cbn. split; intros Heq.
+          * now f_equal.
+          * apply noConfusion_inv in Heq. apply Heq.
+        + intros HYP ι Heq. apply noConfusion_inv in Heq. apply (HYP ι Heq).
+      - cbn - [inst_term]. constructor. intros ι.
+        rewrite inst_pathcondition_app. apply and_iff_compat_r.
+        rewrite inst_formula_eqs_nctx. cbn [inst_term].
+        split; intros Heq.
+        + f_equal. apply Heq.
+        + apply (@f_equal _ _ (@𝑹_unfold R0)) in Heq.
+          rewrite ?𝑹_unfold_fold in Heq. apply Heq.
+    Qed.
+
+    Lemma simplify_formula_spec {Σ} (fml : Formula Σ) (k : List Formula Σ) :
+      OptionSpec
+        (fun fmlsk : List Formula Σ => forall ι, instpc fmlsk ι <-> inst fml ι /\ instpc k ι)
+        (forall ι, ~ inst fml ι)
+        (simplify_formula fml k).
+    Proof.
+      destruct fml; cbn - [peval].
+      - constructor; intros ι. now rewrite inst_pathcondition_cons.
+      - generalize (simplify_formula_bool_spec (peval t) k).
+        apply optionspec_monotonic; cbn; intros; specialize (H ι);
+          now rewrite (peval_sound t) in H.
+      - constructor. intros ι. now rewrite inst_pathcondition_cons.
+      - generalize (simplify_formula_bool_spec (peval (term_binop binop_ge t1 t2)) k).
+        apply optionspec_monotonic; cbn - [peval]; intros; specialize (H ι); revert H;
+          rewrite (peval_sound (term_binop binop_ge t1 t2)); cbn;
+          change (inst_term ?t ?ι) with (inst t ι); unfold is_true;
+          now rewrite Z.geb_le, Z.ge_le_iff.
+      - generalize (simplify_formula_bool_spec (peval (term_binop binop_gt t1 t2)) k).
+        apply optionspec_monotonic; cbn; intros; specialize (H ι); revert H;
+          rewrite (peval_sound (term_binop binop_gt t1 t2)); cbn;
+          change (inst_term ?t ?ι) with (inst t ι); unfold is_true;
+          now rewrite Z.gtb_lt, Z.gt_lt_iff.
+      - generalize (simplify_formula_bool_spec (peval (term_binop binop_le t1 t2)) k).
+        apply optionspec_monotonic; cbn; intros; specialize (H ι); revert H;
+          rewrite (peval_sound (term_binop binop_le t1 t2)); cbn;
+          change (inst_term ?t ?ι) with (inst t ι); unfold is_true;
+          now rewrite Z.leb_le.
+      - generalize (simplify_formula_bool_spec (peval (term_binop binop_lt t1 t2)) k).
+        apply optionspec_monotonic; cbn; intros; specialize (H ι); revert H;
+          rewrite (peval_sound (term_binop binop_lt t1 t2)); cbn;
+          change (inst_term ?t ?ι) with (inst t ι); unfold is_true;
+          now rewrite Z.ltb_lt.
+      - generalize (simplify_formula_eq_spec (peval t1) (peval t2) k).
+        apply optionspec_monotonic; cbn; intros; specialize (H ι);
+          now rewrite (peval_sound t1), (peval_sound t2) in H.
+      - constructor. intros ι. now rewrite inst_pathcondition_cons.
+    Qed.
+
+    Lemma simplify_formulas_spec {Σ} (fmls k : List Formula Σ) :
+      OptionSpec
+        (fun fmlsk : List Formula Σ => forall ι, instpc fmlsk ι <-> instpc fmls ι /\ instpc k ι)
+        (forall ι, ~ instpc fmls ι)
+        (simplify_formulas fmls k).
+    Proof.
+      induction fmls as [|fml fmls]; cbn.
+      - constructor. intuition. constructor.
+      - apply optionspec_bind. revert IHfmls.
+        apply optionspec_monotonic.
+        + intros fmlsk Hfmls.
+          generalize (simplify_formula_spec fml fmlsk).
+          apply optionspec_monotonic.
+          * intros ? Hfml ι. specialize (Hfmls ι). specialize (Hfml ι).
+            rewrite inst_pathcondition_cons. intuition.
+          * intros Hfml ι. specialize (Hfml ι).
+            rewrite inst_pathcondition_cons. intuition.
+        + intros Hfmls ι. specialize (Hfmls ι).
+          rewrite inst_pathcondition_cons. intuition.
+    Qed.
+
+    Definition occurs_check_lt {Σ x} (xIn : x ∈ Σ) {σ} (t : Term Σ σ) : option (Term (Σ - x) σ) :=
+      match t with
+      | @term_var _ y σ yIn =>
+        if Nat.ltb (inctx_at xIn) (inctx_at yIn) then occurs_check xIn t else None
+      | _ => occurs_check xIn t
+      end.
+
+    Lemma occurs_check_lt_sound {Σ x} (xIn : x ∈ Σ) {σ} (t : Term Σ σ) (t' : Term (Σ - x) σ) :
+      occurs_check_lt xIn t = Some t' -> t = subst t' (sub_shift xIn).
+    Proof.
+      unfold occurs_check_lt. intros Heq.
+      refine (occurs_check_sound xIn t (t' := t') _).
+      destruct t; auto.
+      destruct (inctx_at xIn <? inctx_at ςInΣ); auto.
+      discriminate.
+    Qed.
+
+    Equations(noeqns) try_unify_bool {w : World} (t : Term w ty_bool) :
+      option { w' & Tri w w' } :=
+      try_unify_bool (@term_var _ x σ xIn) :=
+        Some (existT _ (tri_cons x (term_lit ty_bool true) tri_id));
+      try_unify_bool (term_not (@term_var _ x σ xIn)) :=
+        Some (existT _ (tri_cons x (term_lit ty_bool false) tri_id));
+      try_unify_bool _ :=
+        None.
+
+    Definition try_unify_eq {w : World} {σ} (t1 t2 : Term w σ) :
+      option { w' & Tri w w' } :=
+      match t1 with
+      | @term_var _ ς σ ςInΣ =>
+        fun t2 : Term w σ =>
+          match occurs_check_lt ςInΣ t2 with
+          | Some t => Some (existT _ (tri_cons ς t tri_id))
+          | None => None
+          end
+      | _ => fun _ => None
+      end t2.
+
+    Definition try_unify_formula {w : World} (fml : Formula w) :
+      option { w' & Tri w w' } :=
+      match fml with
+      | formula_bool t => try_unify_bool t
+      | formula_eq t1 t2 =>
+        match try_unify_eq t1 t2 with
+        | Some r => Some r
+        | None => try_unify_eq t2 t1
+        end
+      | _ => None
+      end.
+
+    Lemma try_unify_bool_spec {w : World} (t : Term w ty_bool) :
+      OptionSpec (fun '(existT w' ν) => forall ι, inst (T := STerm ty_bool) t ι = true <-> inst_triangular ν ι) True (try_unify_bool t).
+    Proof.
+      dependent elimination t; cbn; try constructor; auto.
+      intros ι. cbn. intuition.
+      dependent elimination e0; cbn; try constructor; auto.
+      intros ι. cbn. destruct (ι ‼ ς)%exp; intuition.
+    Qed.
+
+    Lemma try_unify_eq_spec {w : World} {σ} (t1 t2 : Term w σ) :
+      OptionSpec (fun '(existT w' ν) => forall ι, inst t1 ι = inst t2 ι <-> inst_triangular ν ι) True (try_unify_eq t1 t2).
+    Proof.
+      unfold try_unify_eq. destruct t1; cbn; try (constructor; auto; fail).
+      destruct (occurs_check_lt ςInΣ t2) eqn:Heq; constructor; auto.
+      apply occurs_check_lt_sound in Heq. subst.
+      intros ι. rewrite inst_subst, inst_sub_shift.
+      cbn. intuition.
+    Qed.
+
+    Lemma try_unify_formula_spec {w : World} (fml : Formula w) :
+      OptionSpec (fun '(existT w' ν) => forall ι, (inst fml ι : Prop) <-> inst_triangular ν ι) True (try_unify_formula fml).
+    Proof.
+      unfold try_unify_formula; destruct fml; cbn; try (constructor; auto; fail).
+      - apply try_unify_bool_spec.
+      - destruct (try_unify_eq_spec t1 t2) as [[w' ν] HYP|_]. constructor. auto.
+        destruct (try_unify_eq_spec t2 t1) as [[w' ν] HYP|_]. constructor.
+        intros ι. specialize (HYP ι). intuition.
+        now constructor.
+    Qed.
+
+    Definition unify_formula {w0 : World} (fml : Formula w0) :
+      { w1 & Tri w0 w1 * List Formula w1 }%type :=
+      match try_unify_formula fml with
+      | Some (existT w1 ν01) => existT w1 (ν01 , nil)
+      | None => existT w0 (tri_id , cons fml nil)
+      end.
+
+    Lemma unify_formula_spec {w0 : World} (fml : Formula w0) :
+      match unify_formula fml with
+      | existT w1 (ν01 , fmls) =>
+        (forall ι0 : SymInstance w0,
+            inst (A := Prop) fml ι0 ->
+            inst_triangular ν01 ι0 /\
+            instpc fmls (inst (sub_triangular_inv ν01) ι0)) /\
+        (forall ι1 : SymInstance w1,
+            instpc fmls ι1 ->
+            inst (A := Prop) fml (inst (sub_triangular ν01) ι1))
+      end.
+    Proof.
+      unfold unify_formula.
+      destruct (try_unify_formula_spec fml).
+      - destruct a as [w1 ν01]. split.
+        + intros ι0 Hfml. specialize (H ι0). intuition. constructor.
+        + intros ι1 []. apply H. apply inst_triangular_valid.
+      - split; intros ?; rewrite inst_pathcondition_cons;
+          cbn; rewrite inst_sub_id; intuition.
+    Qed.
+
+    Fixpoint unify_formulas {w0 : World} (fmls : List Formula w0) :
+      { w1 & Tri w0 w1 * List Formula w1 }%type.
+    Proof.
+      destruct fmls as [|fml fmls].
+      - exists w0. split. apply tri_id. apply nil.
+      - destruct (unify_formulas w0 fmls) as (w1 & ν01 & fmls1).
+        clear unify_formulas fmls.
+        destruct (unify_formula (persist fml (acc_triangular ν01))) as (w2 & ν12 & fmls2).
+        exists w2. split. apply (tri_comp ν01 ν12).
+        refine (app fmls2 (persist fmls1 (acc_triangular ν12))).
+    Defined.
+
+    Lemma unify_formulas_spec {w0 : World} (fmls0 : List Formula w0) :
+      match unify_formulas fmls0 with
+      | existT w1 (ν01 , fmls1) =>
+        (forall ι0 : SymInstance w0,
+            instpc fmls0 ι0 ->
+            inst_triangular ν01 ι0 /\
+            instpc fmls1 (inst (sub_triangular_inv ν01) ι0)) /\
+        (forall ι1 : SymInstance w1,
+            instpc fmls1 ι1 ->
+            instpc fmls0 (inst (sub_triangular ν01) ι1))
+      end.
+    Proof.
+      induction fmls0 as [|fml0 fmls0]; cbn.
+      - split; intros ι0; rewrite inst_sub_id; intuition.
+      - destruct (unify_formulas fmls0) as (w1 & ν01 & fmls1).
+        pose proof (unify_formula_spec (persist fml0 (acc_triangular ν01))) as IHfml.
+        destruct (unify_formula (persist fml0 (acc_triangular ν01))) as (w2 & ν12 & fmls2).
+        destruct IHfmls0 as [IHfmls01 IHfmls10].
+        destruct IHfml as [IHfml12 IHfml21].
+        split.
+        + intros ι0. rewrite inst_pathcondition_cons. intros [Hfml Hfmls].
+          specialize (IHfmls01 ι0 Hfmls). destruct IHfmls01 as [Hν01 Hfmls1].
+          specialize (IHfml12 (inst (sub_triangular_inv ν01) ι0)).
+          rewrite inst_persist, sub_acc_triangular in IHfml12.
+          rewrite inst_triangular_right_inverse in IHfml12; auto.
+          specialize (IHfml12 Hfml). destruct IHfml12 as [Hν12 Hfmls2].
+          rewrite inst_pathcondition_app, inst_persist, inst_tri_comp, sub_acc_triangular.
+          split; auto. rewrite sub_triangular_inv_comp, inst_subst. split; auto.
+          revert Hfmls1. remember (inst (sub_triangular_inv ν01) ι0) as ι1.
+          rewrite inst_triangular_right_inverse; auto.
+        + intros ι2. rewrite ?inst_pathcondition_app, inst_persist, sub_acc_triangular.
+          intros [Hfmls2 Hfmls1].
+          specialize (IHfml21 ι2 Hfmls2). rewrite inst_persist, sub_acc_triangular in IHfml21.
+          specialize (IHfmls10 (inst (sub_triangular ν12) ι2) Hfmls1).
+          rewrite sub_triangular_comp, inst_subst.
+          rewrite inst_pathcondition_cons. split; auto.
+    Qed.
+
+    Open Scope lazy_bool_scope.
+    Equations(noind) formula_eqb {Σ} (f1 f2 : Formula Σ) : bool :=
+      formula_eqb (formula_bool t1) (formula_bool t2) := Term_eqb t1 t2;
+      formula_eqb (formula_le t11 t12) (formula_le t21 t22) := Term_eqb t11 t21 &&& Term_eqb t12 t22;
+      formula_eqb (formula_lt t11 t12) (formula_lt t21 t22) := Term_eqb t11 t21 &&& Term_eqb t12 t22;
+      formula_eqb (formula_ge t11 t12) (formula_ge t21 t22) := Term_eqb t11 t21 &&& Term_eqb t12 t22;
+      formula_eqb (formula_gt t11 t12) (formula_gt t21 t22) := Term_eqb t11 t21 &&& Term_eqb t12 t22;
+      formula_eqb (@formula_eq _ σ t11 t12) (@formula_eq _ τ t21 t22) with eq_dec σ τ => {
+        formula_eqb (@formula_eq _ σ t11 t12) (@formula_eq _ ?(σ) t21 t22) (left eq_refl) :=
+          Term_eqb t11 t21 &&& Term_eqb t12 t22;
+        formula_eqb (@formula_eq _ σ t11 t12) (@formula_eq _ τ t21 t22) (right _) := false
+      };
+      formula_eqb (@formula_neq _ σ t11 t12) (@formula_neq _ τ t21 t22) with eq_dec σ τ => {
+        formula_eqb (@formula_neq _ σ t11 t12) (@formula_neq _ ?(σ) t21 t22) (left eq_refl) :=
+          Term_eqb t11 t21 &&& Term_eqb t12 t22;
+        formula_eqb (@formula_neq _ σ t11 t12) (@formula_neq _ τ t21 t22) (right _) := false
+      };
+      formula_eqb (@formula_user _ p ts1) (@formula_user _ q ts2) with 𝑷_eq_dec p q => {
+        formula_eqb (@formula_user _ p ts1) (@formula_user _ ?(p) ts2) (left eq_refl) :=
+          env_eqb_hom (@Term_eqb _) ts1 ts2;
+        formula_eqb (@formula_user _ p ts1) (@formula_user _ q ts2) (right _) := false
+      };
+      formula_eqb _ _ := false.
+
+    Lemma formula_eqb_spec {Σ} (f1 f2 : Formula Σ) :
+      BoolSpec (f1 = f2) True (formula_eqb f1 f2).
+    Proof.
+      induction f1; dependent elimination f2;
+        simp formula_eqb;
+        try (constructor; auto; fail).
+      - destruct 𝑷_eq_dec.
+        + destruct e; cbn.
+          destruct (env_eqb_hom_spec (@Term_eqb Σ) (@Term_eqb_spec Σ) ts ts0);
+            constructor; intuition.
+        + now constructor.
+      - destruct (Term_eqb_spec t t0); constructor; intuition.
+      - repeat
+          match goal with
+          | |- context[Term_eqb ?t1 ?t2] =>
+              destruct (Term_eqb_spec t1 t2); cbn;
+              try (constructor; intuition; fail)
+          end.
+      - repeat
+          match goal with
+          | |- context[Term_eqb ?t1 ?t2] =>
+              destruct (Term_eqb_spec t1 t2); cbn;
+              try (constructor; intuition; fail)
+          end.
+      - repeat
+          match goal with
+          | |- context[Term_eqb ?t1 ?t2] =>
+              destruct (Term_eqb_spec t1 t2); cbn;
+              try (constructor; intuition; fail)
+          end.
+      - repeat
+          match goal with
+          | |- context[Term_eqb ?t1 ?t2] =>
+              destruct (Term_eqb_spec t1 t2); cbn;
+              try (constructor; intuition; fail)
+          end.
+      - destruct (eq_dec σ σ0); cbn.
+        + destruct e.
+          repeat
+            match goal with
+            | |- context[Term_eqb ?t1 ?t2] =>
+              destruct (Term_eqb_spec t1 t2); cbn;
+                try (constructor; intuition; fail)
+            end.
+        + constructor; auto.
+      - destruct (eq_dec σ σ1); cbn.
+        + destruct e.
+          repeat
+            match goal with
+            | |- context[Term_eqb ?t1 ?t2] =>
+              destruct (Term_eqb_spec t1 t2); cbn;
+                try (constructor; intuition; fail)
+            end.
+        + constructor; auto.
+    Qed.
+
+    Fixpoint assumption_formula {Σ} (pc : PathCondition Σ) (fml : Formula Σ) (k : List Formula Σ) {struct pc} : List Formula Σ :=
+      match pc with
+      | nil       => cons fml k
+      | cons f pc => if formula_eqb f fml
+                     then k
+                     else assumption_formula pc fml k
+      end.
+
+    Fixpoint assumption_formulas {Σ} (pc : PathCondition Σ) (fmls : List Formula Σ) (k : List Formula Σ) {struct fmls} : List Formula Σ :=
+      match fmls with
+      | nil           => k
+      | cons fml fmls => assumption_formula pc fml (assumption_formulas pc fmls k)
+      end.
+
+    Lemma assumption_formula_spec {Σ} (pc : PathCondition Σ) (fml : Formula Σ) (k : List Formula Σ) (ι : SymInstance Σ) :
+      instpc pc ι -> inst (A := Prop) fml ι /\ instpc k ι <-> instpc (assumption_formula pc fml k) ι.
+    Proof.
+      induction pc as [|f pc]; cbn.
+      - now rewrite inst_pathcondition_cons.
+      - rewrite inst_pathcondition_cons.
+        intros [Hf Hpc]. specialize (IHpc Hpc).
+        destruct (formula_eqb_spec f fml);
+          subst; intuition.
+    Qed.
+
+    Lemma assumption_formulas_spec {Σ} (pc : PathCondition Σ) (fmls : List Formula Σ) (k : List Formula Σ) (ι : SymInstance Σ) :
+      instpc pc ι -> instpc fmls ι /\ instpc k ι <-> instpc (assumption_formulas pc fmls k) ι.
+    Proof.
+      intros Hpc. induction fmls as [|fml fmls]; cbn.
+      - intuition. constructor.
+      - rewrite inst_pathcondition_cons.
+        pose proof (assumption_formula_spec pc fml (assumption_formulas pc fmls k) ι Hpc).
+        intuition.
+    Qed.
+
+    Definition solver_generic_round : Solver :=
+      fun w0 fmls0 =>
+        match simplify_formulas fmls0 nil with
+        | Some fmls01 => Some (unify_formulas (assumption_formulas (wco w0) fmls01 nil))
+        | None => None
+        end.
+
+    Lemma solver_generic_round_spec : SolverSpec solver_generic_round.
+    Proof.
+      unfold solver_generic_round. intros w0 fmls0.
+      destruct (simplify_formulas_spec fmls0 nil) as [fmls0' Hequiv|].
+      - constructor.
+        pose proof (unify_formulas_spec (assumption_formulas (wco w0) fmls0' nil)) as Hunify.
+        destruct (unify_formulas (assumption_formulas (wco w0) fmls0' nil)) as (w1 & ν01 & fmls1).
+        intros ι0 Hpc0. specialize (Hequiv ι0).
+        pose proof (assumption_formulas_spec (wco w0) fmls0' nil ι0 Hpc0) as Hassumption.
+        destruct Hassumption as [Hassumption01 Hassumption10].
+        destruct Hunify as [Hunify01 Hunify10]. specialize (Hunify01 ι0).
+        split.
+        + intros Hfmls0. apply Hunify01. apply Hassumption01.
+          split. apply Hequiv. split; auto. constructor.
+          constructor.
+        + intros ι1 Heqι. specialize (Hunify10 ι1).
+          split.
+          * intros Hfmls0. destruct Hequiv as [_ Hequiv].
+            inster Hequiv by split; auto; constructor.
+            inster Hassumption01 by split; auto; constructor.
+            inster Hunify01 by auto. destruct Hunify01 as [Hν01 Hfmls1].
+            revert Hfmls1. subst. now rewrite inst_triangular_left_inverse.
+          * intros Hfmls1. inster Hunify10 by subst; auto.
+            apply Hequiv. apply Hassumption10. subst; auto.
+      - constructor. intuition.
+    Qed.
+
+    Definition solver_compose (s1 s2 : Solver) : Solver :=
+      fun w0 fmls0 =>
+        option_bind
+          (fun '(existT w1 (ν01 , fmls1)) =>
+             option_map
+               (fun '(existT w2 (ν12 , fmls2)) =>
+                  existT w2 (tri_comp ν01 ν12 , fmls2))
+               (s2 _ fmls1)) (s1 _ fmls0).
+
+    Lemma solver_compose_spec {s1 s2} (spec1 : SolverSpec s1) (spec2 : SolverSpec s2) : SolverSpec (solver_compose s1 s2).
+    Proof.
+      unfold SolverSpec, solver_compose. intros w0 fmls0.
+      apply optionspec_bind.
+      generalize (spec1 _ fmls0); clear spec1.
+      apply optionspec_monotonic; auto.
+      intros (w1 & ν01 & fmls1) H1.
+      apply optionspec_map.
+      generalize (spec2 _ fmls1); clear spec2.
+      apply optionspec_monotonic; auto.
+      - intros (w2 & ν12 & fmls2) H2. intros ι0 Hpc0.
+        specialize (H1 ι0 Hpc0). destruct H1 as [H01 H10].
+        rewrite inst_tri_comp. split.
+        + intros Hfmls0. split; auto.
+          remember (inst (sub_triangular_inv ν01) ι0) as ι1.
+          assert (instpc (wco w1) ι1) as Hpc1 by
+              (subst; apply entails_triangular_inv; auto).
+          apply H2; auto. apply H10; auto.
+          subst; rewrite inst_triangular_right_inverse; auto.
+        + intros ι2 Hpc2 Hι0. rewrite sub_triangular_comp, inst_subst in Hι0.
+          remember (inst (sub_triangular ν12) ι2) as ι1.
+          assert (instpc (wco w1) ι1) as Hpc1 by
+              (revert Hpc2; subst; rewrite <- sub_acc_triangular, <- inst_persist; apply ent_acc).
+          rewrite H10; eauto. apply H2; auto.
+      - intros Hfmls1 ι0 Hpc0 Hfmls0. specialize (H1 ι0 Hpc0).
+        destruct H1 as [H01 H10]. inster H01 by auto.
+        pose (inst (sub_triangular_inv ν01) ι0) as ι1.
+        assert (instpc (wco w1) ι1) as Hpc1 by
+            (subst; apply entails_triangular_inv; auto).
+        apply (Hfmls1 ι1 Hpc1). revert Hfmls0.
+        apply H10; auto. subst ι1.
+        now rewrite inst_triangular_right_inverse.
+    Qed.
+
+    Definition solver_generic (solver_user : Solver) : Solver :=
+      solver_compose solver_generic_round (solver_compose solver_user solver_generic_round).
+
+    Lemma solver_generic_spec {solver_user} (H : SolverSpec solver_user) :
+      SolverSpec (solver_generic solver_user).
+    Proof.
+      unfold solver_generic.
+      auto using solver_compose_spec, solver_generic_round_spec.
+    Qed.
+
+    Definition null : Solver :=
+      fun w fmls => Some (existT w (tri_id , fmls)).
+
+    Lemma null_spec : SolverSpec null.
+    Proof.
+      intros w fmls. constructor. cbn. intros ι Hpc. split. auto.
+      intros ι' Hpc' ->. now rewrite inst_sub_id.
+    Qed.
+
+  End Solver.
+
   Inductive Assertion (Σ : LCtx) : Type :=
   | asn_formula (fml : Formula Σ)
   | asn_chunk (c : Chunk Σ)
@@ -1228,252 +2265,8 @@ Module Assertions
 
   Arguments interpret_assertion {_ _ _} _ _.
 
-  Section Worlds.
 
-    Record World : Type :=
-      MkWorld
-        { wctx :> LCtx;
-          wco  : PathCondition wctx;
-        }.
 
-    Definition wnil : World := @MkWorld ctx_nil nil.
-    Definition wsnoc (w : World) (b : 𝑺 * Ty) : World :=
-      @MkWorld (wctx w ▻ b) (subst (wco w) sub_wk1).
-    Definition wformula (w : World) (f : Formula w) : World :=
-      @MkWorld (wctx w) (cons f (wco w)).
-    Definition wsubst (w : World) x {σ} {xIn : x :: σ ∈ w} (t : Term (w - (x :: σ)) σ) : World :=
-      {| wctx := wctx w - (x :: σ); wco := subst (wco w) (sub_single xIn t) |}.
-    Global Arguments wsubst w x {σ xIn} t.
-    Definition wcat (w : World) (Δ : LCtx) : World :=
-      @MkWorld (wctx w ▻▻ Δ) (subst (wco w) (sub_cat_left Δ)).
-    Definition wformulas (w : World) (fmls : List Formula w) : World :=
-      @MkWorld (wctx w) (app fmls (wco w)).
-
-    Definition TYPE : Type := World -> Type.
-    Bind Scope modal with TYPE.
-    Definition Valid (A : TYPE) : Type :=
-      forall w, A w.
-    Definition Impl (A B : TYPE) : TYPE :=
-      fun w => A w -> B w.
-    Definition Forall {I : Type} (A : I -> TYPE) : TYPE :=
-      fun w => forall i : I, A i w.
-    (* Definition Cat (A : TYPE) (Δ : LCtx) : TYPE := *)
-    (*   fun w => A (wcat w Δ). *)
-
-  End Worlds.
-
-  Section TriangularSubstitutions.
-
-    Ltac rew := rewrite ?subst_sub_comp, ?subst_shift_single, ?subst_sub_id, ?sub_comp_id_right,
-        ?sub_comp_id_left, ?inst_sub_id, ?inst_sub_id.
-
-    Inductive Tri (w : World) : World -> Type :=
-    | tri_id        : Tri w w
-    | tri_cons {w' x σ}
-        (xIn : (x::σ) ∈ w) (t : Term (wctx w - (x::σ)) σ)
-        (ν : Tri (wsubst w x t) w') : Tri w w'.
-    Global Arguments tri_id {_}.
-    Global Arguments tri_cons {_ _} x {_ _} t ν.
-
-    Fixpoint tri_comp {w1 w2 w3} (ν12 : Tri w1 w2) : Tri w2 w3 -> Tri w1 w3 :=
-      match ν12 with
-      | tri_id           => fun ν => ν
-      | tri_cons x t ν12 => fun ν => tri_cons x t (tri_comp ν12 ν)
-      end.
-
-    Fixpoint sub_triangular {w1 w2} (ζ : Tri w1 w2) : Sub w1 w2 :=
-      match ζ with
-      | tri_id         => sub_id _
-      | tri_cons x t ζ => subst (sub_single _ t) (sub_triangular ζ)
-      end.
-
-    Lemma sub_triangular_comp {w0 w1 w2} (ν01 : Tri w0 w1) (ν12 : Tri w1 w2) :
-      sub_triangular (tri_comp ν01 ν12) =
-      subst (sub_triangular ν01) (sub_triangular ν12).
-    Proof.
-      induction ν01; cbn [sub_triangular tri_comp].
-      - now rew.
-      - now rewrite sub_comp_assoc, IHν01.
-    Qed.
-
-    Fixpoint sub_triangular_inv {w1 w2} (ζ : Tri w1 w2) : Sub w2 w1 :=
-      match ζ with
-      | tri_id         => sub_id _
-      | tri_cons x t ζ => subst (sub_triangular_inv ζ) (sub_shift _)
-      end.
-
-    Lemma sub_triangular_inv_comp {w0 w1 w2} (ν01 : Tri w0 w1) (ν12 : Tri w1 w2) :
-      sub_triangular_inv (tri_comp ν01 ν12) =
-      subst (sub_triangular_inv ν12) (sub_triangular_inv ν01).
-    Proof.
-      induction ν01; cbn.
-      - now rew.
-      - now rewrite IHν01, sub_comp_assoc.
-    Qed.
-
-    Fixpoint inst_triangular {w0 w1} (ζ : Tri w0 w1) (ι : SymInstance w0) : Prop :=
-      match ζ with
-      | tri_id => True
-      | @tri_cons _ Σ' x σ xIn t ζ0 =>
-        let ι' := env_remove (x :: σ) ι xIn in
-        env_lookup ι xIn = inst t ι' /\ inst_triangular ζ0 ι'
-      end.
-
-    Lemma inst_triangular_left_inverse {w1 w2 : World} (ι2 : SymInstance w2) (ν : Tri w1 w2) :
-      inst (sub_triangular_inv ν) (inst (sub_triangular ν) ι2) = ι2.
-    Proof. rewrite <- inst_subst. induction ν; cbn - [subst]; now rew. Qed.
-
-    Lemma inst_triangular_right_inverse {w1 w2 : World} (ι1 : SymInstance w1) (ζ : Tri w1 w2) :
-      inst_triangular ζ ι1 ->
-      inst (sub_triangular ζ) (inst (sub_triangular_inv ζ) ι1) = ι1.
-    Proof.
-      intros Hζ. induction ζ; cbn - [subst].
-      - now rew.
-      - cbn in Hζ. rewrite <- inst_sub_shift in Hζ. destruct Hζ as [? Hζ].
-        rewrite ?inst_subst, IHζ, inst_sub_single_shift; auto.
-    Qed.
-
-    (* Forward entailment *)
-    Lemma entails_triangular_inv {w0 w1} (ν : Tri w0 w1) (ι0 : SymInstance w0) :
-      inst_triangular ν ι0 ->
-      instpc (wco w0) ι0 ->
-      instpc (wco w1) (inst (sub_triangular_inv ν) ι0).
-    Proof.
-      induction ν; cbn.
-      - cbn. rewrite inst_sub_id. auto.
-      - rewrite <- inst_sub_shift, inst_subst. intros [Heqx Heq'] Hpc0.
-        apply IHν; cbn; auto.
-        rewrite inst_subst, inst_sub_single_shift; auto.
-    Qed.
-
-    Lemma inst_triangular_valid {w0 w1} (ζ01 : Tri w0 w1) (ι1 : SymInstance w1) :
-      inst_triangular ζ01 (inst (sub_triangular ζ01) ι1).
-    Proof.
-      induction ζ01; cbn; auto.
-      rewrite <- inst_lookup, lookup_sub_comp. rewrite lookup_sub_single_eq.
-      rewrite <- inst_sub_shift. rewrite <- ?inst_subst.
-      rewrite subst_sub_comp.
-      rewrite subst_shift_single.
-      split; auto.
-      rewrite <- ?sub_comp_assoc.
-      rewrite sub_comp_shift_single.
-      rewrite sub_comp_id_left.
-      auto.
-    Qed.
-
-    Lemma inst_tri_comp {w0 w1 w2} (ν01 : Tri w0 w1) (ν12 : Tri w1 w2) (ι0 : SymInstance w0) :
-      inst_triangular (tri_comp ν01 ν12) ι0 <->
-      inst_triangular ν01 ι0 /\ inst_triangular ν12 (inst (sub_triangular_inv ν01) ι0).
-    Proof.
-      induction ν01; cbn.
-      - rewrite inst_sub_id; intuition.
-      - rewrite ?inst_subst, ?inst_sub_shift. split.
-        + intros (Heq & Hwp). apply IHν01 in Hwp. now destruct Hwp.
-        + intros ([Heq Hν01] & Hwp). split; auto. apply IHν01; auto.
-    Qed.
-
-  End TriangularSubstitutions.
-
-  Definition Solver : Type :=
-    forall {w0 : World} (fmls0 : List Formula w0),
-      option { w1 & Tri w0 w1 * List Formula w1 }%type.
-
-  Definition SolverSpec (s : Solver) : Prop :=
-    forall {w0 : World} (fmls0 : List Formula w0),
-      OptionSpec
-        (fun '(existT w1 (ζ, fmls1)) =>
-           forall ι0,
-             instpc (wco w0) ι0 ->
-             (instpc fmls0 ι0 -> inst_triangular ζ ι0) /\
-               (forall ι1,
-                   instpc (wco w1) ι1 ->
-                   ι0 = inst (sub_triangular ζ) ι1 ->
-                   instpc fmls0 ι0 <-> inst fmls1 ι1))
-        (forall ι, instpc (wco w0) ι -> ~ instpc fmls0 ι)
-        (s w0 fmls0).
-
-  Definition SoundSolver : Type :=
-    { s : Solver | SolverSpec s }.
-
-  Section Accessibility.
-
-    Import Entailment.
-
-    Inductive Acc (w1 : World) : World -> Type :=
-    | acc_refl : Acc w1 w1
-    | acc_sub {w2 : World} (ζ : Sub w1 w2) (ent : wco w2 ⊢ subst (wco w1) ζ) : Acc w1 w2.
-    Global Arguments acc_refl {w} : rename.
-    Global Arguments acc_sub {w1 w2} ζ ent.
-    Notation "w1 ⊒ w2" := (Acc w1 w2) (at level 80).
-
-    Equations(noeqns) acc_trans {w0 w1 w2} (ω01 : w0 ⊒ w1) (ω12 : w1 ⊒ w2) : w0 ⊒ w2 :=
-    | acc_refl         | ω12              := ω12;
-    | ω01              | acc_refl         := ω01;
-    | acc_sub ζ01 ent1 | acc_sub ζ12 ent2 := acc_sub (subst (T := Sub _) ζ01 ζ12) _.
-    Next Obligation.
-      intros w0 w1 w2 ζ01 Hpc01 ζ12 Hpc12. transitivity (subst (wco w1) ζ12); auto.
-      rewrite subst_sub_comp. now apply proper_subst_entails.
-    Qed.
-    Global Arguments acc_trans {w0 w1 w2} !ω01 !ω12.
-
-    Definition sub_acc {w1 w2} (ω : w1 ⊒ w2) : Sub (wctx w1) (wctx w2) :=
-      match ω with
-      | acc_refl    => sub_id _
-      | acc_sub ζ _ => ζ
-      end.
-
-    Lemma sub_acc_trans {w0 w1 w2} (ω01 : w0 ⊒ w1) (ω12 : w1 ⊒ w2) :
-      sub_acc (acc_trans ω01 ω12) = subst (sub_acc ω01) (sub_acc ω12).
-    Proof.
-      destruct ω01, ω12; cbn - [subst];
-        now rewrite ?sub_comp_id_left, ?sub_comp_id_right.
-    Qed.
-
-    Definition Box (A : TYPE) : TYPE :=
-      fun w0 => forall w1, w0 ⊒ w1 -> A w1.
-
-  End Accessibility.
-
-  Instance preorder_acc : CRelationClasses.PreOrder Acc :=
-    CRelationClasses.Build_PreOrder Acc (@acc_refl) (@acc_trans).
-
-  Declare Scope modal.
-  Delimit Scope modal with modal.
-
-  Module ModalNotations.
-
-    Notation "⊢ A" := (Valid A%modal) (at level 100).
-    Notation "A -> B" := (Impl A%modal B%modal) : modal.
-    Notation "□ A" := (Box A%modal) (at level 9, format "□ A", right associativity) : modal.
-    Notation "⌜ A ⌝" := (fun (w : World) => Const A%type w) (at level 0, format "⌜ A ⌝") : modal.
-    Notation "'∀' x .. y , P " :=
-      (Forall (fun x => .. (Forall (fun y => P%modal)) ..))
-        (at level 99, x binder, y binder, right associativity)
-      : modal.
-    Notation "w1 ⊒ w2" := (Acc w1 w2) (at level 80).
-
-  End ModalNotations.
-  Import ModalNotations.
-  Open Scope modal.
-
-  Definition K {A B} :
-    ⊢ □(A -> B) -> (□A -> □B) :=
-    fun w0 f a w1 ω01 =>
-      f w1 ω01 (a w1 ω01).
-  Definition T {A} :
-    ⊢ □A -> A :=
-    fun w0 a => a w0 acc_refl.
-  Definition four {A} :
-    ⊢ □A -> □□A :=
-    fun w0 a w1 ω01 w2 ω12 =>
-      a w2 (acc_trans ω01 ω12).
-  Arguments four : simpl never.
-
-  (* faster version of (four _ sub_wk1) *)
-  (* Definition four_wk1 {A} : *)
-  (*   ⊢ □A -> ∀ b, Snoc (□A) b := *)
-  (*   fun w0 a b w1 ω01 => a w1 (env_tail ω01). *)
-  (* Arguments four_wk1 {A Σ0} pc0 a b [Σ1] ζ01 : rename. *)
 
   Module SymProp.
 
@@ -1959,7 +2752,6 @@ Module Assertions
   End SymProp.
   Notation SymProp := SymProp.SymProp.
   Notation 𝕊 := SymProp.SymProp.
-  Import SymProp.
 
 End Assertions.
 
@@ -1973,6 +2765,8 @@ Module Type SymbolicContractKit
   Parameter Inline CEnv   : SepContractEnv.
   Parameter Inline CEnvEx : SepContractEnvEx.
   Parameter Inline LEnv   : LemmaEnv.
-  Parameter solver_user   : option SoundSolver.
+
+  Parameter solver_user      : Solver.
+  Parameter solver_user_spec : SolverSpec solver_user.
 
 End SymbolicContractKit.
